Safety commit progress so far on example `time_protection` instantation
Signed-off-by: Scott Buckley <sbuckley@anchorage.keg.cse.unsw.edu.au>

proof/infoflow/timeprotection/MemSysExample_Generic32Bit_A.thy
@@ -12,29 +12,162 @@ begin
   - L1-D (write-through)
   - L2 (write-back) *)
 
-(* Recall this is just for the L2 cache. *)
-definition collision_set_A :: "address \<Rightarrow> address set" where
-  "collision_set_A a = {a}" (* TODO *)
+record other_state_A =
+  mem :: "address \<Rightarrow> machine_word"
+
+record regs_A =
+  r0 :: "machine_word"
+
+(* This part is all just for the L2 cache. *)
+(* Note: There should be "x" mask bits for an "x word" type, and the offset
+   should match the number of zeroes to the right of the mask. *)
+type_synonym tag_A = "22 word"
+definition tag_mask :: address where "tag_mask = 0b11111111111111111111110000000000"
+definition tag_offset :: nat where "tag_offset = 10"
+type_synonym index_A = "6 word"
+definition index_mask :: address where "index_mask = 0b1111110000"
+definition index_offset :: nat where "index_offset = 4"
+type_synonym colour_A = "2 word"
+definition colour_mask :: address where "colour_mask = 0b1100000000"
+definition colour_offset :: nat where "colour_offset = 8"
+
+definition tag_of :: "address \<Rightarrow> tag_A" where
+  "tag_of a = ucast ((a AND tag_mask) >> tag_offset)"
+definition index_of :: "address \<Rightarrow> index_A" where
+  "index_of a = ucast ((a AND index_mask) >> index_offset)"
+definition colour_of :: "address \<Rightarrow> colour_A" where
+  "colour_of a = ucast ((a AND colour_mask) >> colour_offset)"
+
+(* In this system let's choose to have the max number of user domains possible on the hardware
+   - that is, as many as there are colours. -robs. *)
+type_synonym userdomain_A = colour_A
+abbreviation addr_colour_A :: "address \<Rightarrow> colour_A" where "addr_colour_A \<equiv> colour_of"
+abbreviation colour_userdomain_A :: "colour_A \<Rightarrow> userdomain_A" where "colour_userdomain_A \<equiv> id"
+
+definition collides_in_pch_A :: "address rel" where
+  "collides_in_pch_A = {(a, a'). colour_of a = colour_of a' \<and> tag_of a = tag_of a'}"
 
 (* As our cache impact model is not distinguishing yet between I-cache and D-cache nor counting
-   timing impacts of instruction fetching itself, let's say fch is just the L1-D. *)
-type_synonym fch_cachedness_A = bool
-type_synonym pch_cachedness_A = bool
+   timing impacts of instruction fetching itself, let's say fch is just the L1-D.
+   Also a big TODO here still is to distinguish between virtual and physical addresses. *)
+
+datatype writethru_cachedness = WT_Absent | WT_Valid
+datatype writeback_cachedness = WB_Absent | WB_Valid | WB_DirtyValid
+
+type_synonym fch_cachedness_A = writethru_cachedness
+type_synonym pch_cachedness_A = writeback_cachedness
 type_synonym fch_A = "fch_cachedness_A fch"
 type_synonym pch_A = "pch_cachedness_A pch"
 
-definition read_impact_A :: "(fch_A, pch_A) cache_impact" where
-  "read_impact_A a f p = (f, p)" (* TODO *)
+definition fch_read_impact_A :: "fch_A fch_impact" where
+  "fch_read_impact_A a f = f" (* TODO *)
 
-definition write_impact_A :: "(fch_A, pch_A) cache_impact" where
-  "write_impact_A a f p = (f, p)" (* TODO *)
+definition pch_read_impact_A :: "(fch_A, pch_A) pch_impact" where
+  "pch_read_impact_A a f p = p" (* TODO *)
 
-interpretation time_protection_A: time_protection collision_set_A read_impact_A write_impact_A
-  apply unfold_locales
-   (* pch_partitioned_read *)
-   defer
-  (* pch_partitioned_write *)
-  defer
+definition fch_write_impact_A :: "fch_A fch_impact" where
+  "fch_write_impact_A a f = f" (* TODO *)
+
+definition pch_write_impact_A :: "(fch_A, pch_A) pch_impact" where
+  "pch_write_impact_A a f p = p" (* TODO *)
+
+definition read_cycles_A :: "fch_cachedness_A \<Rightarrow> pch_cachedness_A \<Rightarrow> time" where
+  "read_cycles_A a p = 0" (* TODO *)
+
+definition write_cycles_A :: "fch_cachedness_A \<Rightarrow> pch_cachedness_A \<Rightarrow> time" where
+  "write_cycles_A a p = 0" (* TODO *)
+
+definition do_read_A :: "address \<Rightarrow> other_state_A \<Rightarrow> regs_A \<Rightarrow> regs_A" where
+  "do_read_A a s r = r" (* TODO *)
+
+definition do_write_A :: "address \<Rightarrow> other_state_A \<Rightarrow> regs_A \<Rightarrow> other_state_A" where
+  "do_write_A a s r = s" (* TODO *)
+
+definition store_time_A :: "time \<Rightarrow> regs_A \<Rightarrow> regs_A" where
+  "store_time_A t r = r" (* TODO *)
+
+definition padding_regs_impact_A :: "time \<Rightarrow> regs_A \<Rightarrow> regs_A" where
+  "padding_regs_impact_A t r = r"  (* TODO *)
+
+definition empty_fch_A :: fch_A where
+  "empty_fch_A a = WT_Absent"
+
+definition fch_flush_cycles_A:: "fch_A \<Rightarrow> time" where
+  "fch_flush_cycles_A f = 0" (* TODO *)
+
+definition do_pch_flush_A :: "pch_A \<Rightarrow> address set \<Rightarrow> pch_A" where
+  "do_pch_flush_A p as = p" (* TODO *)
+
+definition addr_domain_A :: "address \<Rightarrow> userdomain_A domain" where
+  "addr_domain_A a = Sched" (* TODO *)
+
+lemma colours_not_shared_A:
+  "colour_userdomain_A c1 \<noteq> colour_userdomain_A c2 \<Longrightarrow> c1 \<noteq> c2"
+  using distinct_lemma by blast
+
+lemma no_cross_colour_collisions_A:
+  "(a1, a2) \<in> collides_in_pch_A \<Longrightarrow> addr_colour_A a1 = addr_colour_A a2"
+  using collides_in_pch_A_def by blast
+
+lemma addr_domain_valid_A:
+  "addr_domain_A a = Sched \<or> addr_domain_A a = User (colour_userdomain_A (addr_colour_A a))"
+  oops (* TODO: Define addr_domain_A first. *)
+
+definition current_domain_A :: "other_state_A \<Rightarrow> userdomain_A domain" where
+  "current_domain_A s = Sched" (* TODO *)
+
+definition external_uwr_A :: "userdomain_A domain \<Rightarrow> (other_state_A \<times> other_state_A) set" where
+  "external_uwr_A d = UNIV" (* TODO *)
+
+lemma external_uwr_equiv_rel_A:
+  "equiv UNIV (external_uwr_A d)"
   oops
+
+lemma external_uwr_same_domain_A:
+  "(s1, s2) \<in> external_uwr_A d \<Longrightarrow> current_domain_A s1 = current_domain_A s2"
+  oops
+
+lemma do_write_maintains_external_uwr_out_A:
+  "addr_domain_A a \<noteq> d \<and> addr_domain_A a \<noteq> Sched \<Longrightarrow>
+   (s, do_write_A a s r) \<in> external_uwr_A d"
+  oops
+
+lemma do_write_maintains_external_uwr_in:
+  "addr_domain_A a = d \<or> addr_domain_A a = Sched \<Longrightarrow>
+   (s, t) \<in> external_uwr_A d \<Longrightarrow>
+   (do_write_A a s r, do_write_A a t r) \<in> external_uwr_A d"
+  oops
+
+definition pch_flush_cycles_A :: "pch_A \<Rightarrow> address set \<Rightarrow> time" where
+  "pch_flush_cycles_A p as = 0" (* TODO *)
+
+definition touched_addrs_A :: "other_state_A \<Rightarrow> address set" where
+  "touched_addrs_A s = {}" (* TODO *)
+
+lemma external_uwr_same_touched_addrs_A:
+  "(s1, s2) \<in> external_uwr_A d \<Longrightarrow> current_domain_A s1 = d \<Longrightarrow>
+   touched_addrs_A s1 = touched_addrs_A s2"
+  oops
+
+definition can_domain_switch_A :: "other_state_A \<Rightarrow> bool" where
+  "can_domain_switch_A s = False" (* TODO *)
+
+lemma can_domain_switch_public_A:
+  "(s1, s2) \<in> external_uwr_A d \<Longrightarrow> can_domain_switch_A s1 = can_domain_switch_A s2"
+  oops
+
+interpretation time_protection_A: time_protection collides_in_pch_A
+  fch_read_impact_A pch_read_impact_A
+  fch_write_impact_A pch_write_impact_A
+  read_cycles_A write_cycles_A
+  do_read_A do_write_A
+  store_time_A padding_regs_impact_A
+  empty_fch_A fch_flush_cycles_A do_pch_flush_A
+  addr_domain_A addr_colour_A colour_userdomain_A
+  current_domain_A external_uwr_A pch_flush_cycles_A touched_addrs_A can_domain_switch_A
+  apply unfold_locales
+  oops
+(* Gerwin's feedback: at least get to the end of this once
+   so we know it's satisfiable even if not flexible *)
 
 end
